unity/safety.lean
@@ -16,80 +16,161 @@ open temporal
 
 class has_safety (α : Type u) : Type (u+1) :=
   (σ : Type)
+  (init : α → pred' σ)
   (step : α → σ → σ → Prop)
 
-def state := has_safety.σ
+section has_safety
 
-def step {α} [has_safety α] : α → state α → state α → Prop :=
-has_safety.step
+parameter (α : Type u)
+parameter [has_safety α]
+parameter s : α
 
-def unless {α} [has_safety α] (s : α) (p q : pred' (state α)) : Prop
-:= ∀ σ σ', step s σ σ' → p σ ∧ ¬ q σ → p σ' ∨ q σ'
+def state := has_safety.σ α
 
-def co {α} [has_safety α] (s : α) (p q : pred' (state α)) : Prop
-:= ∀ σ σ', step s σ σ' → p σ → q σ'
+parameter {α}
 
-def co' {α} [has_safety α] (s : α) (r : act (state α)) : Prop
-:= ∀ σ σ', step s σ σ' → r σ σ'
+def first : pred' state :=
+has_safety.init s
 
-def unless' {α} [has_safety α] (s : α) (p q : pred' (state α)) (e : act (state α)) : Prop
-:= ∀ σ σ', step s σ σ' → ¬ e σ σ' → p σ ∧ ¬ q σ → p σ' ∨ q σ'
+def init (p : pred' state) : Prop :=
+first ⟹ p
 
-lemma unless_eq_unless_except {α} [has_safety α] (s : α) (p q : pred' (state α))
-: unless s p q = unless' s p q (λ _, False) :=
+def step : state → state → Prop :=
+has_safety.step s
+
+inductive reachable : state → Prop
+  | init : ∀ σ, first σ → reachable σ
+  | step : ∀ σ σ', reachable σ → step σ σ' → reachable σ'
+
+def holds (p : pred' state) : Prop :=
+reachable ⟹ p
+
+local prefix `⊢ `:40 := holds
+
+lemma relative {p : pred' state}
+  (h : ⦃ p ⦄)
+: ⊢ p :=
+by { intros σ h', apply h }
+
+lemma holds_imp_holds {p q : pred' state}
+  (h  : ⊢ p ⟶ q)
+  (hp : ⊢ p)
+: ⊢ q :=
+begin
+  intros σ hr,
+  apply h _ hr,
+  apply hp _ hr,
+end
+
+lemma holds_imp_and {p q r : pred' state}
+  (h  : ⊢ p ⟶ q)
+  (hp : ⊢ p ⟶ r)
+: ⊢ p ⟶ q && r :=
+sorry
+
+@[simp]
+lemma holds_True
+: ⊢ True :=
+entails_True _
+
+@[refl]
+lemma holds_impl_refl {p : pred' state}
+: ⊢ p ⟶ p :=
+relative (entails_refl _)
+
+@[trans]
+lemma holds_impl_trans {p : pred' state} (q : pred' state) {r : pred' state}
+  (hp : ⊢ p ⟶ q)
+  (hq : ⊢ q ⟶ r)
+: ⊢ p ⟶ r :=
+begin
+  apply holds_imp_holds _ _ hq,
+  apply holds_imp_holds _ _ hp,
+  apply relative s _,
+  intro, apply p_imp_p_imp_p_imp_left,
+end
+
+def unless (p q : pred' state) : Prop
+:= ∀ σ σ', reachable σ → step σ σ' → p σ ∧ ¬ q σ → p σ' ∨ q σ'
+
+def co (p q : pred' state) : Prop
+:= ∀ σ σ', reachable σ → step σ σ' → p σ → q σ'
+
+def co'  (r : act state) : Prop
+:= ∀ σ σ', reachable σ → step σ σ' → r σ σ'
+
+def invariant (p : pred' state) : Prop :=
+init p ∧ co p p
+
+parameter {s}
+lemma invariant_holds {p : pred' state}
+  (h : invariant p)
+: ⊢ p :=
+begin
+  intros σ hr,
+  induction hr with σ h' σ σ' h' IH,
+  { apply h.left _ h' },
+  { apply h.right _ _ h' IH ih_1, },
+end
+parameter s
+
+def unless' (p q : pred' state) (e : act state) : Prop
+:= ∀ σ σ', reachable σ → step σ σ' → ¬ e σ σ' → p σ ∧ ¬ q σ → p σ' ∨ q σ'
+
+lemma unless_eq_unless_except (p q : pred' state)
+: unless p q = unless' p q (λ _, False) :=
 begin
   unfold unless unless',
   apply forall_congr_eq, intro σ,
   apply forall_congr_eq, intro σ',
   apply forall_congr_eq, intro P,
+  apply forall_congr_eq, intro P,
   generalize (p σ ∧ ¬q σ → p σ' ∨ q σ') r,
-  simp,
-  intro,
-  rw [-iff_eq_eq],
-  split
-  ; intro hr ; intros
-  ; apply hr,
-  trivial,
+  intro,   simp [iff_eq_eq],
+  begin [smt] eblast end,
 end
 
-def saf_ex {α} [has_safety α] (s : α) : cpred (state α) :=
- ([] ⟦ step s ⟧)
+def saf_ex: cpred state :=
+ •(has_safety.init s) && [] ⟦ step ⟧
 
 section properties
 
 open predicate
 
-parameter {α : Type u}
-variable [has_safety α]
-variable s : α
-def σ := state α
+def σ := state
 
-lemma unless_action {α} [has_safety α] {s : α} {p q : pred' (state α)}
-  (h : unless s p q)
-: ⟦ λ σ σ', (p σ ∧ ¬ q σ) ⟧ ⟹ ( ⟦ step s ⟧ ⟶  ⟦ λ _, p || q ⟧ ) :=
+parameters {α s}
+lemma unless_action {p q : pred' state}
+  (h : unless p q)
+: •reachable ⟹ ( ⟦ λ σ σ', (p σ ∧ ¬ q σ) ⟧ ⟶ ( ⟦ step ⟧ ⟶  ⟦ λ _, p || q ⟧ ) ) :=
 begin
   intros τ,
   unfold temporal.action,
-  intros hpnq act,
-  apply h _ _ act hpnq
+  intros R hpnq act,
+  apply h _ _ R act hpnq
 end
 
-lemma impl_unless {p q : pred' σ} (h : p ⟹ q) : unless s p q :=
+lemma impl_unless' {p q : pred' σ} (h : ⊢ p ⟶ q) : unless p q :=
 begin
-  intros σ σ' h₀ h₁,
+  intros σ σ' hr h₀ h₁,
   cases h₁ with h₁ h₂,
-  cases h₂ (h _ h₁)
+  cases h₂ (h _ hr h₁)
 end
+
+lemma impl_unless {p q : pred' σ} (h : p ⟹ q) : unless p q :=
+by { apply impl_unless', apply relative _ h }
 
 lemma unless_weak_rhs {p q r : pred' σ}
          (h : q ⟹ r)
-         (P₀ : unless s p q)
-         : unless s p r :=
+         (P₀ : unless p q)
+         : unless p r :=
 begin
   apply forall_imp_forall _ P₀,
   intro s,
   apply forall_imp_forall _,
   intro s',
+  apply imp_imp_imp_right' _,
+  intro step,
   apply imp_imp_imp_right' _,
   intro step,
   apply imp_mono,
@@ -101,13 +182,13 @@ begin
 end
 
 lemma unless_conj_gen {p₀ q₀ p₁ q₁ : pred' σ}
-         (P₀ : unless s p₀ q₀)
-         (P₁ : unless s p₁ q₁)
-         : unless s (p₀ && p₁) ((q₀ && p₁) || (p₀ && q₁) || (q₀ && q₁)) :=
+  (P₀ : unless p₀ q₀)
+  (P₁ : unless p₁ q₁)
+: unless (p₀ && p₁) ((q₀ && p₁) || (p₀ && q₁) || (q₀ && q₁)) :=
 begin
-  intros s s' step H,
-  note P₀ := P₀ s s' step,
-  note P₁ := P₁ s s' step,
+  intros s s' R step H,
+  note P₀ := P₀ s s' R step,
+  note P₁ := P₁ s s' R step,
   cases H with H₀ H₂,
   cases H₀ with Hp₀ Hp₁,
   simp [not_or_iff_not_and_not,not_and_iff_not_or_not] at H₂,
@@ -132,12 +213,12 @@ begin
     exact ⟨P₀,P₁⟩ },
 end
 
-theorem unless_conj {p₀ q₀ p₁ q₁ : pred' (state α)}
-  (h₀ : unless s p₀ q₀)
-  (h₁ : unless s p₁ q₁)
-: unless s (p₀ && p₁) (q₀ || q₁) :=
+theorem unless_conj {p₀ q₀ p₁ q₁ : pred' σ}
+  (h₀ : unless p₀ q₀)
+  (h₁ : unless p₁ q₁)
+: unless (p₀ && p₁) (q₀ || q₁) :=
 begin
-  apply unless_weak_rhs _ _ (unless_conj_gen _ h₀ h₁),
+  apply unless_weak_rhs _ (unless_conj_gen h₀ h₁),
   apply p_or_entails_of_entails,
   apply p_or_p_imp_p_or',
   { apply p_and_elim_left },
@@ -146,11 +227,11 @@ begin
 end
 
 lemma unless_disj_gen {p₀ q₀ p₁ q₁ : pred' σ}
-         (P₀ : unless s p₀ q₀)
-         (P₁ : unless s p₁ q₁)
-         : unless s (p₀ || p₁) ((q₀ && - p₁) || (- p₀ && q₁) || (q₀ && q₁)) :=
+         (P₀ : unless p₀ q₀)
+         (P₁ : unless p₁ q₁)
+         : unless (p₀ || p₁) ((q₀ && - p₁) || (- p₀ && q₁) || (q₀ && q₁)) :=
 begin
-  intros σ σ' STEP h,
+  intros σ σ' R STEP h,
   cases h with h₀ h₁,
   rw [p_not_eq_not,p_not_p_or,p_not_p_or] at h₁,
   repeat { rw p_not_p_and at h₁ },
@@ -158,13 +239,8 @@ begin
   cases h₁ with h₁ h₂, cases h₂ with h₂ h₃,
   simp at h₀,
   assert h₄ : p₀ σ ∧ ¬q₀ σ ∨ p₁ σ ∧ ¬q₁ σ,
-  { note h₄ := and.intro h₀ h₁,
-    rw -distrib_right_or at h₄,
-    note h₅ := and.intro h₂ h₃,
-    rw [or_comm,-distrib_right_or] at h₅,
-    rw [distrib_left_or],
-    exact ⟨h₄,h₅⟩, },
-  note STEP₀ := or.imp (P₀ _ _ STEP) (P₁ _ _ STEP) h₄,
+  { clear STEP R P₀ P₁, begin [smt] by_cases p₀ σ, by_cases (q₀ σ) end },
+  note STEP₀ := or.imp (P₀ _ _ R STEP) (P₁ _ _ R STEP) h₄,
   assert STEP₁ : (p₀ σ' ∨ p₁ σ') ∨ q₀ σ' ∨ q₁ σ',
   { revert STEP₀,
     apply iff.mp, simp, },
@@ -182,11 +258,11 @@ begin
 end
 
 lemma unless_disj' {p₀ q₀ p₁ q₁ : pred' σ}
-         (P₀ : unless s p₀ q₀)
-         (P₁ : unless s p₁ q₁)
-         : unless s (p₀ || p₁) (q₀ || q₁) :=
+         (P₀ : unless p₀ q₀)
+         (P₁ : unless p₁ q₁)
+         : unless (p₀ || p₁) (q₀ || q₁) :=
 begin
-  note h := unless_disj_gen _ P₀ P₁, revert h,
+  note h := unless_disj_gen P₀ P₁, revert h,
   apply unless_weak_rhs,
   intros i,
   apply or.rec,
@@ -202,55 +278,55 @@ begin
     apply and.elim_left },
 end
 
-lemma unless_refl (p : pred' (state α)) : unless s p p :=
+lemma unless_refl (p : pred' σ) : unless p p :=
 begin
   apply impl_unless,
   apply λ _, id
 end
 
-lemma unless_antirefl (p : pred' (state α)) : unless s p (-p) :=
+lemma unless_antirefl (p : pred' σ) : unless p (-p) :=
 begin
-  intros σ σ' X h,
+  intros σ σ' R X h,
   apply classical.em,
 end
 
-lemma True_unless (p : pred' (state α)) : unless s True p :=
+lemma True_unless (p : pred' σ) : unless True p :=
 begin
-  intros σ σ' X h,
+  intros σ σ' R X h,
   left, trivial
 end
 
-lemma unless_cancellation {p q r : pred' (state α)}
-  (S₀ : unless s p q)
-  (S₁ : unless s q r)
-: unless s (p || q) r :=
+lemma unless_cancellation {p q r : pred' σ}
+  (S₀ : unless p q)
+  (S₁ : unless q r)
+: unless (p || q) r :=
 begin
-  intros σ σ' h,
+  intros σ σ' R h,
   rw and_shunting,
   intros h₀ hr,
   rw [p_or_comm,-p_or_not_and,p_and_comm] at h₀,
   cases h₀ with hq hpnq,
-  { apply or.imp_left (or.intro_right _) (S₁ _ _ h _),
+  { apply or.imp_left (or.intro_right _) (S₁ _ _ R h _),
     exact ⟨hq,hr⟩ },
   { left,
-    apply S₀ _ _ h hpnq, }
+    apply S₀ _ _ R h hpnq, }
 end
 
-lemma exists_unless {t} {p : t → pred' (state α)} {q : pred' (state α)}
-  (h : ∀ i, unless s (p i) q)
-: unless s (∃∃ i, p i) q :=
+lemma exists_unless {t} {p : t → pred' σ} {q : pred' σ}
+  (h : ∀ i, unless (p i) q)
+: unless (∃∃ i, p i) q :=
 begin
-  intros σ σ' STEP,
+  intros σ σ' R STEP,
   apply and.rec,
   intros h₀ h₁, cases h₀ with x h₀,
-  note h₂ := h x _ _ STEP ⟨h₀,h₁⟩,
+  note h₂ := h x _ _ R STEP ⟨h₀,h₁⟩,
   apply or.imp_left _ h₂,
   apply Exists.intro x,
 end
 
-lemma forall_unless_exists_str {n} {p q : fin n → pred' (state α)}
-  (h : ∀ i, unless s (p i) (p i && q i))
-: unless s (∀∀ i, p i) ( (∀∀ i, p i) && (∃∃ i, q i) ) :=
+lemma forall_unless_exists_str {n} {p q : fin n → pred' σ}
+  (h : ∀ i, unless (p i) (p i && q i))
+: unless (∀∀ i, p i) ( (∀∀ i, p i) && (∃∃ i, q i) ) :=
 begin
   revert p q h,
   induction n with n IH
@@ -259,17 +335,17 @@ begin
   { rw [p_exists_split_one,p_forall_split_one],
     assert h' : ∀ i, unless s (restr p i) (restr p i && restr q i),
     { unfold restr, intro i, apply h },
-    note Hconj := unless_conj_gen _ (h fin.max) (IH h'),
-    apply unless_weak_rhs _ _ Hconj, clear Hconj,
+    note Hconj := unless_conj_gen (h fin.max) (IH h'),
+    apply unless_weak_rhs _ Hconj, clear Hconj,
     { intro, simp, clear h h' IH,
       generalize (∀ (x : fin n), restr p x i) PP, intro,
       generalize (∃ (x : fin n), restr q x i) QQ, intro,
-      begin [smt] by_cases (p fin.max i), by_cases PP, by_cases QQ, eblast end, } },
+      begin [smt] by_cases (p fin.max i), by_cases PP, by_cases QQ end, } },
 end
 
-lemma forall_unless_exists {n} {p q : fin n → pred' (state α)}
-  (h : ∀ i, unless s (p i) (q i))
-: unless s (∀∀ i, p i) (∃∃ i, q i) :=
+lemma forall_unless_exists {n} {p q : fin n → pred' σ}
+  (h : ∀ i, unless (p i) (q i))
+: unless (∀∀ i, p i) (∃∃ i, q i) :=
 begin
   revert p q h,
   induction n with n IH
@@ -278,27 +354,78 @@ begin
   { rw [p_exists_split_one,p_forall_split_one],
     assert h' : ∀ i, unless s (restr p i) (restr q i),
     { unfold restr, intro i, apply h },
-    note Hconj := unless_conj_gen _ (h fin.max) (IH h'),
-    apply unless_weak_rhs _ _ Hconj, clear Hconj,
+    note Hconj := unless_conj_gen (h fin.max) (IH h'),
+    apply unless_weak_rhs _ Hconj, clear Hconj,
     { intro, simp,
       begin [smt] by_cases (q fin.max i), eblast end, } },
 end
 
-lemma forall_unless {n} {p : fin n → pred' (state α)} {b : pred' (state α)}
-  (h : ∀ i, unless s (p i) b)
-: unless s (∀∀ i, p i) b :=
+lemma forall_unless {n} {p : fin n → pred' σ} {b : pred' σ}
+  (h : ∀ i, unless (p i) b)
+: unless (∀∀ i, p i) b :=
 begin
-  note h : unless s (∀∀ i, p i) (∃∃ i : fin n, b) := forall_unless_exists _ h,
-  apply unless_weak_rhs _ _ h,
+  note h : unless s (∀∀ i, p i) (∃∃ i : fin n, b) := forall_unless_exists h,
+  apply unless_weak_rhs _ h,
   intro x, simp, apply Exists.rec _,
   intro , apply id,
 end
 
 open nat temporal stream
 
+lemma henceforth_reachable  {τ : stream state}
+    (sem : saf_ex τ)
+: [] •reachable $ τ :=
+begin
+  intro i,
+  simp [init_drop],
+  induction i with i IH,
+  { apply reachable.init _ (sem.left), },
+  { apply reachable.step _ _ IH,
+    note H := sem.right i,
+    rw action_drop at H,
+    apply H },
+end
+
+lemma henceforth_inv {τ : stream state} {p : pred' state}
+  (sem : saf_ex τ)
+  (h : invariant p)
+: []• p $ τ :=
+begin
+  note H := henceforth_reachable sem,
+  revert H,
+  apply henceforth_entails_henceforth,
+  apply init_entails_init,
+  apply invariant_holds h,
+end
+
+lemma assume_reach_step {τ : stream σ} {A : act σ}
+  (sem : saf_ex τ)
+  (h : ∀ s s', reachable s → step s s' → A s s')
+: [] ⟦ A ⟧ $ τ :=
+begin
+  apply henceforth_imp_henceforth _ sem.right,
+  apply henceforth_entails_henceforth _ _ (henceforth_reachable sem),
+  unfold p_entails,
+  rw [-p_and_p_imp,init_eq_action,action_and_action],
+  apply action_entails_action,
+  simp [and_shunting],
+  apply h,
+end
+
+lemma assume_reach_step' {τ : stream σ} {A : act σ}
+  (sem : saf_ex τ)
+  (h : ∀ s s', reachable s → reachable s' → step s s' → A s s')
+: [] ⟦ A ⟧ $ τ :=
+begin
+  apply assume_reach_step sem,
+  intros σ σ' Hr Hs,
+  apply h _ _ Hr _ Hs,
+  apply reachable.step _ _ Hr Hs,
+end
+
 lemma unless_sem' {τ : stream σ} {p q : pred' σ} (i : ℕ)
-    (sem : saf_ex s τ)
-    (H : unless s p q)
+    (sem : saf_ex τ)
+    (H : unless p q)
 : (<>•p) (τ.drop i) → (<>[]•p) (τ.drop i) ∨ (<>•q) (τ.drop i) :=
 begin
   intros h,
@@ -312,13 +439,13 @@ begin
     simp [stream.drop_drop],
     simp [stream.drop_drop] at hp,
     assert GOAL : ⟦λ (_x : σ), p || q⟧ (drop (i + (j + k)) τ),
-    { apply unless_action H,
+    { apply unless_action H _ (henceforth_reachable sem _),
       { simp [action_drop], split,
         simp [init_drop] at hp, simp [init_drop,hp],
         note hnq := henceforth_str' (k+j) H',
         simp [not_init,drop_drop,init_drop] at hnq,
         simp [hnq,init_to_fun], },
-      { apply sem } },
+      { apply sem.right } },
     unfold action at GOAL,
     cases GOAL with hp hq,
     { unfold action,
@@ -328,45 +455,51 @@ begin
       apply hp },
     { note hnq' := henceforth_str' (k+j+1) H',
       unfold action,
-      simp [drop_drop,not_init] at hnq',
+      simp [drop_drop,not_init,init_drop] at hnq',
       unfold drop init at hq hnq',
-      simp at hnq' hq,
+      simp at hq,
       cases hnq' hq } }
 end
 
 lemma co_sem'  {τ : stream σ} {A : act σ}
-    (sem : saf_ex s τ)
-    (H : co' s A)
+    (sem : saf_ex τ)
+    (H : co' A)
 : []⟦ A ⟧ $ τ :=
 begin
+  note H := henceforth_reachable sem,
+  note H' := sem.right,
+  revert H',
+  apply henceforth_imp_henceforth,
+  revert H,
   unfold saf_ex at sem,
-  apply henceforth_entails_henceforth _ _ sem,
-  apply action_entails_action,
-  apply H
+  apply henceforth_entails_henceforth _ _ ,
+  rw [init_eq_action],
+  intros τ h,
+  apply H _ _ h
 end
 
 lemma unless_sem {τ : stream σ} {p q : pred' σ}
-    (sem : saf_ex s τ)
-    (H : unless s p q)
+    (sem : saf_ex τ)
+    (H : unless p q)
 : (<>•p) τ → (<>[]•p) τ ∨ (<>•q) τ :=
 by apply @unless_sem' _ _ _ _ _ _ 0 sem H
 
 lemma unless_sem_str {τ : stream σ} {p q : pred' σ}
-    (sem : saf_ex s τ)
-    (H : unless s p q)
+    (sem : saf_ex τ)
+    (H : unless p q)
 : ([]<>•p ⟶ <>[]•p || []<>•q) τ :=
 begin
   rw [shunting,-eventually_eventually ([] _),not_eventually,-henceforth_and],
   apply henceforth_imp_henceforth, intro j,
   rw [-shunting],
-  note H' := unless_sem' _ j sem H,
+  note H' := unless_sem' j sem H,
   apply H'
 end
 
 
 lemma unless_sem_exists' {τ : stream σ} {t} {p : t → pred' σ} {q : pred' σ} {evt : act σ}
-    (sem : saf_ex s τ)
-    (H : ∀ x, unless' s (p x) q evt)
+    (sem : saf_ex τ)
+    (H : ∀ x, unless' (p x) q evt)
 : ( []<>(∃∃ x, •p x) ⟶ (∃∃ x, <>[]•p x) || []<>(•q || ⟦ evt ⟧) ) τ :=
 begin
   intro H₀,
@@ -399,7 +532,8 @@ begin
     note H₃ := H₁ (j+k+1),
     simp [drop_drop,init_to_fun] at H₃,
     simp [not_or_iff_not_and_not,init_to_fun] at H₂,
-    note IH := H x σ _ (sem _) H₂.right ⟨ih_1,H₂.left⟩,
+    note Hr := henceforth_reachable sem,
+    note IH := H x σ _ (Hr _) (sem.right _) H₂.right ⟨ih_1,H₂.left⟩,
     cases IH with IH IH,
     { apply IH },
     { unfold drop at H₃ IH,
@@ -409,12 +543,12 @@ begin
 end
 
 lemma unless_sem_exists {τ : stream σ} {t} {p : t → pred' σ} {q : pred' σ}
-    (sem : saf_ex s τ)
-    (H : ∀ x, unless s (p x) q)
+    (sem : saf_ex τ)
+    (H : ∀ x, unless (p x) q)
 : ( []<>(∃∃ x, •p x) ⟶ (∃∃ x, <>[]•p x) || []<>•q ) τ :=
 begin
   assert H₀ : ( []<>(∃∃ x, •p x) ⟶ (∃∃ x, <>[]•p x) || []<>(•q || ⟦ λ _, False ⟧) ) τ,
-  { apply unless_sem_exists' _ sem,
+  { apply unless_sem_exists' sem,
     simp [unless_eq_unless_except] at H,
     apply H, },
   assert H₁ : action (λ _, False) = (False : cpred σ),
@@ -425,5 +559,9 @@ begin
 end
 
 end properties
+
+end has_safety
+
+infix ` ⊢ `:40 := holds
 
 end unity
